

Force as the Gradient of PE

Consider a particle acted on by  $\vec{F}(\vec{r})$  (conservative) with PE  $U(\vec{r})$ . Let's look at how much work is done by  $\vec{F}$  in a small displacement:  $\vec{r} \rightarrow \vec{r} + d\vec{r}$

$$\begin{aligned} W(\vec{r} \rightarrow \vec{r} + d\vec{r}) &= \vec{F}(\vec{r}) \cdot d\vec{r} \quad \rightarrow \quad d\vec{r} = dx \hat{x} + dy \hat{y} + dz \hat{z} \\ &= F_x dx + F_y dy + F_z dz \end{aligned}$$

Also:

$$\begin{aligned} W(\vec{r} \rightarrow \vec{r} + d\vec{r}) &= - [U(\vec{r} + d\vec{r}) - U(\vec{r})] \equiv dU \\ &= - [U(x+dx, y+dy, z+dz) - U(x, y, z)] \end{aligned}$$

Note: for  $f(x)$  of one variable, one can write

$$df = f(x+dx) - f(x) = \frac{df}{dx} dx$$

For a fn of 3 variables, we have instead:

$$\begin{aligned} dU &= U(x+dx, y+dy, z+dz) - U(x, y, z) \\ &= \frac{\partial U}{\partial x} dx + \frac{\partial U}{\partial y} dy + \frac{\partial U}{\partial z} dz \\ &\quad \uparrow \quad \quad \uparrow \quad \quad \nearrow \\ &\quad \text{partial derivatives} \end{aligned}$$

$$W(\vec{r} \rightarrow \vec{r} + d\vec{r}) = dU$$

$$\begin{aligned} W(\vec{r} \rightarrow \vec{r} + d\vec{r}) &= - \left[ \frac{\partial U}{\partial x} dx + \frac{\partial U}{\partial y} dy + \frac{\partial U}{\partial z} dz \right] \\ &= F_x dx + F_y dy + F_z dz \end{aligned}$$

$$\Rightarrow F_x = -\frac{\partial U}{\partial x}, \quad F_y = -\frac{\partial U}{\partial y}, \quad F_z = -\frac{\partial U}{\partial z}$$

$$\vec{F} = -\frac{\partial U}{\partial x} \hat{x} - \frac{\partial U}{\partial y} \hat{y} - \frac{\partial U}{\partial z} \hat{z}$$

Remember:  $\vec{\nabla} f = \frac{\partial f}{\partial x} \hat{x} + \frac{\partial f}{\partial y} \hat{y} + \frac{\partial f}{\partial z} \hat{z}$

$$\Rightarrow \boxed{\vec{F} = -\vec{\nabla} U}$$

One can derive  $\vec{F}$  from  $U$ !!

You can think of  $\vec{\nabla}$  as an operator:

$$\vec{\nabla} = \hat{x} \frac{\partial}{\partial x} + \hat{y} \frac{\partial}{\partial y} + \hat{z} \frac{\partial}{\partial z}$$

$$\left[ \text{then } \vec{\nabla} f = \hat{x} \frac{\partial}{\partial x} f + \hat{y} \frac{\partial}{\partial y} f + \hat{z} \frac{\partial}{\partial z} f \quad \text{as usual} \right]$$

$$\begin{aligned} \text{We can see that } dU &= \frac{\partial U}{\partial x} dx + \frac{\partial U}{\partial y} dy + \frac{\partial U}{\partial z} dz \\ &= \vec{\nabla} U \cdot d\vec{r} \end{aligned}$$

$$\text{Thus for any function, } df = \vec{\nabla} \cdot d\vec{r} \quad \& \quad \text{in 1D, this reduces to } df = \frac{df}{dx} dx$$

---

The 2<sup>nd</sup> condition that  $\vec{F}$  is conservative:

The work done by a force  $\vec{F}$  is path-independent iff:

$$\vec{\nabla} \times \vec{F} = 0$$

"the curl of  $\vec{F}$ "

$$\begin{aligned} \text{If } \vec{\nabla} &= \hat{x}_1 \frac{\partial}{\partial x_1} + \hat{y}_2 \frac{\partial}{\partial y_2} + \hat{z}_3 \frac{\partial}{\partial z_3} \quad \text{and } \vec{F} = F_x \hat{x}_1 + F_y \hat{y}_2 + F_z \hat{z}_3, \quad \text{then } \vec{\nabla} \times \vec{F} \text{ is just a} \\ &= \hat{x}_1 \frac{\partial}{\partial x_1} + \hat{x}_2 \frac{\partial}{\partial x_2} + \hat{x}_3 \frac{\partial}{\partial x_3} = \hat{x}_i \frac{\partial}{\partial x_i} \quad = F_1 \hat{x}_1 + F_2 \hat{x}_2 + F_3 \hat{x}_3 = F_i \hat{x}_i \\ &\quad \text{cross product} \end{aligned}$$

$$(\vec{\nabla} \times \vec{F})_i = \epsilon_{ijk} \frac{\partial}{\partial x_j} F_k \quad \text{just like } (\vec{A} \times \vec{B})_i = \epsilon_{ijk} A_j B_k$$

$$\vec{\nabla} \times \vec{F} = \left( \frac{\partial F_z}{\partial y} - \frac{\partial F_y}{\partial z} \right) \hat{x} + \left( \frac{\partial F_x}{\partial z} - \frac{\partial F_z}{\partial x} \right) \hat{y} + \left( \frac{\partial F_y}{\partial x} - \frac{\partial F_x}{\partial y} \right) \hat{z}$$

Example: Is  $F_g = mg \hat{z}$  conservative?

$$\vec{\nabla} \times \vec{F} = \frac{\partial}{\partial y} F_z \hat{x} - \frac{\partial}{\partial x} F_z \hat{y}, \quad F_z = mg$$

$$= 0 - 0 = 0 \quad \Rightarrow \text{yes } \checkmark$$

Is  $F_G = \frac{GmM}{r^2} \hat{r}$  conservative?

$$= \frac{GmM (\hat{r})}{r^2} = \frac{GmM \vec{r}}{r^3} = \frac{GmM (x\hat{x}^1 + y\hat{y}^1 + z\hat{z}^1)}{(x^2+y^2+z^2)^{3/2}} = \frac{GmM x_a \hat{x}_a}{(x_l x_l)^{3/2}}$$

$$(\vec{\nabla} \times \vec{F})_i = \epsilon_{ijk} \frac{\partial}{\partial x_j} F_k = \epsilon_{ijk} \frac{\partial}{\partial x_j} \left[ \frac{GmM x_k}{(x_l x_l)^{3/2}} \right]$$

$$= GmM \epsilon_{ijk} \left[ \frac{\partial x_k}{\partial x_j} \frac{1}{(x_l x_l)^{3/2}} + x_k \frac{\partial}{\partial x_j} (x_l x_l)^{-3/2} \right]$$

$$= GmM \underbrace{\epsilon_{ijk}}_{\substack{=0 \\ \text{if } j=k}} \left[ \underbrace{\delta_{jk}}_{\substack{=0 \\ \text{if } j \neq k}} \frac{1}{(x_l x_l)^{3/2}} + x_k (-3/2) (x_l x_l)^{-5/2} \left( \underbrace{\frac{\partial x_l}{\partial x_j} x_l + x_l \frac{\partial x_l}{\partial x_j}}_{= 2x_l \frac{\partial x_l}{\partial x_j}} \right) \right]$$

$$= GmM \epsilon_{ijk} \left[ 0 - \frac{3}{2} \frac{x_k}{(x_l x_l)^{5/2}} (2x_l \delta_{lj}) \right]$$

$$= -3GmM \epsilon_{ijk} \frac{x_k}{(x_l x_l)^{5/2}} (x_j)$$

$$= -3GmM \frac{\epsilon_{ijk} x_j x_k}{(x_l x_l)^{5/2}}$$

We know  $\epsilon_{ijk} x_j x_k = 0$

Why?  $\epsilon_{ijk} x_j x_k = \epsilon_{ikj} x_k x_j = \epsilon_{ikj} x_j x_k$

rename  
j → k  
k → j

$$\epsilon_{ijk} x_j x_k = \epsilon_{ikj} x_j x_k \quad \text{switch } j \leftrightarrow k \quad \epsilon_{ijk} = -\epsilon_{ikj}$$

$$\epsilon_{ijk} x_j x_k = -\epsilon_{ijk} x_j x_k \Rightarrow \text{must } = 0$$

$$\left( \text{only } \# \text{ st. } n = -n \text{ is } n=0 \right)$$

$$\Rightarrow (\vec{\nabla} \times \vec{F}_G)_i = \frac{-3GmM \epsilon_{ijk} x_j x_k}{(x_l x_l)^{5/2}} = 0 \Rightarrow \text{conservative!}$$